Chop and Change. Tidy.

DataflowNatSemantics.v
@@ -5,9 +5,6 @@ Require Import SynchronousNat.
 
 Definition history := PM.t stream.
 
-Definition find_node (f : ident) : global -> option node :=
-  List.find (fun n=> ident_eqb n.(n_name) f).
-
 Inductive sem_var (H: history)(x: ident)(n: nat)(v: value): Prop :=
 | Sv:
     forall xs,
@@ -243,26 +240,5 @@ Proof.
     specialize H0 with n (xs n).
     apply H0.
     reflexivity.
-Qed.
-
-Lemma find_node_Exists:
-  forall f G, find_node f G <> None <-> List.Exists (fun n=> f = n.(n_name)) G.
-Proof.
-  induction G as [|node G IH].
-  - split; intro Hfn.
-    exfalso; apply Hfn; reflexivity.
-    apply List.Exists_nil in Hfn; contradiction.
-  - destruct (ident_eq_dec node.(n_name) f) as [He|Hne]; simpl.
-    + assert (He' := He); apply BinPos.Pos.eqb_eq in He'.
-      unfold ident_eqb; rewrite He'.
-      split; intro HH; [clear HH|discriminate 1].
-      constructor.
-      symmetry; exact He.
-    + assert (Hne' := Hne); apply BinPos.Pos.eqb_neq in Hne'.
-      unfold ident_eqb; rewrite Hne'.
-      split; intro HH; [ apply IH in HH; constructor 2; exact HH |].
-      apply List.Exists_cons in HH.
-      destruct HH as [HH|HH]; [symmetry in HH; contradiction|].
-      apply IH; exact HH.
 Qed.
 
