DataflowSyntax.v
@@ -1,4 +1,8 @@
 Require Import Rustre.Common.
+Require Import PArith.
+
+Import List.ListNotations.
+Open Scope list_scope.
 
 (** * Dataflow language *)
 
@@ -47,6 +51,9 @@ Record node : Type := mk_node {
   n_eqs : list equation }.
 
 Definition global := list node.
+
+Definition find_node (f : ident) : global -> option node :=
+  List.find (fun n=> ident_eqb n.(n_name) f).
 
 (** ** Predicates *)
 
@@ -826,4 +833,134 @@ Inductive Is_instance_in_eq : ident -> equation -> Prop :=
 
 Definition Is_instance_in (x: ident) (eqs: list equation) : Prop :=
   List.Exists (Is_instance_in_eq x) eqs.
+
+
+Lemma not_Is_node_in_cons:
+  forall n eq eqs,
+    ~ Is_node_in n (eq::eqs) <-> ~Is_node_in_eq n eq /\ ~Is_node_in n eqs.
+Proof.
+  intros n eq eqs.
+  split; intro HH.
+  - split; intro; apply HH; unfold Is_node_in; intuition.
+  - destruct HH; inversion_clear 1; intuition.
+Qed.
+
+Lemma Ordered_nodes_append:
+  forall G G',
+    Ordered_nodes (G ++ G')
+    -> Ordered_nodes G'.
+Proof.
+  induction G as [|nd G IH]; [intuition|].
+  intros G' HnGG.
+  apply IH; inversion_clear HnGG; assumption.
+Qed.
+
+Lemma find_node_Exists:
+  forall f G, find_node f G <> None <-> List.Exists (fun n=> f = n.(n_name)) G.
+Proof.
+  induction G as [|node G IH].
+  - split; intro Hfn.
+    exfalso; apply Hfn; reflexivity.
+    apply List.Exists_nil in Hfn; contradiction.
+  - destruct (ident_eq_dec node.(n_name) f) as [He|Hne]; simpl.
+    + assert (He' := He); apply BinPos.Pos.eqb_eq in He'.
+      unfold ident_eqb; rewrite He'.
+      split; intro HH; [clear HH|discriminate 1].
+      constructor.
+      symmetry; exact He.
+    + assert (Hne' := Hne); apply BinPos.Pos.eqb_neq in Hne'.
+      unfold ident_eqb; rewrite Hne'.
+      split; intro HH; [ apply IH in HH; constructor 2; exact HH |].
+      apply List.Exists_cons in HH.
+      destruct HH as [HH|HH]; [symmetry in HH; contradiction|].
+      apply IH; exact HH.
+Qed.
+
+Lemma find_node_tl:
+  forall f node G,
+    node.(n_name) <> f
+    -> find_node f (node::G) = find_node f G.
+Proof.
+  intros f node G Hnf.
+  unfold find_node.
+  unfold List.find at 1.
+  apply Pos.eqb_neq in Hnf.
+  unfold ident_eqb.
+  rewrite Hnf.
+  reflexivity.
+Qed.
+
+Lemma find_node_split:
+  forall f G node,
+    find_node f G = Some node
+    -> exists bG aG,
+      G = bG ++ node :: aG.
+Proof.
+  induction G as [|nd G IH]; [unfold find_node, List.find; discriminate|].
+  intro nd'.
+  intro Hfind.
+  unfold find_node in Hfind; simpl in Hfind.
+  destruct (ident_eqb (n_name nd) f) eqn:Heq.
+  - injection Hfind; intro He; rewrite <-He in *; clear Hfind He.
+    exists []; exists G; reflexivity.
+  - apply IH in Hfind.
+    destruct Hfind as [bG [aG Hfind]].
+    exists (nd::bG); exists aG; rewrite Hfind; reflexivity.
+Qed.
+
+Lemma Ordered_nodes_cons_find_node_None:
+  forall node G,
+    Ordered_nodes (node::G)
+    -> find_node node.(n_name) G = None.
+Proof.
+  intros node G Hord.
+  inversion_clear Hord as [|? ? Hord' H0 Hfa]; clear H0.
+  induction G as [|eq G IH]; [trivial|].
+  simpl.
+  destruct (ident_eqb eq.(n_name) node.(n_name)) eqn:Heq;
+    apply Forall_cons2 in Hfa;
+    destruct Hfa as [Hneq H0].
+  - apply Peqb_true_eq in Heq.
+    rewrite Heq in Hneq.
+    exfalso; apply Hneq; reflexivity.
+  - apply IH; inversion_clear Hord'; assumption.
+Qed.
+
+Lemma find_node_later_names_not_eq:
+  forall f nd G nd',
+    Ordered_nodes (nd::G)
+    -> find_node f (G) = Some nd'
+    -> f <> nd.(n_name).
+Proof.
+  intros f nd G nd' Hord Hfind.
+  pose proof (Ordered_nodes_cons_find_node_None _ _ Hord) as Hnone.
+  intro Heq.
+  rewrite Heq, Hnone in Hfind.
+  discriminate.
+Qed.
+
+Lemma find_node_later_not_Is_node_in:
+  forall f nd G nd',
+    Ordered_nodes (nd::G)
+    -> find_node f (G) = Some nd'
+    -> ~Is_node_in nd.(n_name) nd'.(n_eqs).
+Proof.
+  intros f nd G nd' Hord Hfind Hini.
+  apply find_node_split in Hfind.
+  destruct Hfind as [bG [aG HG]].
+  rewrite HG in Hord.
+  inversion_clear Hord as [|? ? Hord' H0 Hnin]; clear H0.
+  apply Ordered_nodes_append in Hord'.
+  inversion_clear Hord' as [| ? ? Hord Heqs Hnin'].
+  apply Heqs in Hini.
+  destruct Hini as [H0 HH]; clear H0.
+  rewrite Forall_app in Hnin.
+  destruct Hnin as [H0 Hnin]; clear H0.
+  inversion_clear Hnin as [|? ? H0 HH']; clear H0.
+  apply List.Exists_exists in HH.
+  destruct HH as [node [HaG Heq]].
+  rewrite List.Forall_forall in HH'.
+  apply HH' in HaG.
+  contradiction.
+Qed.
 
